New definition of a post-crash modality (previous definition almost certainly can't work)

src/CSL/Crash.v
@@ -17,50 +17,85 @@ Section crash.
 Context {OpT: Type -> Type}.
 Context `{Λ: Layer OpT} `{irisG OpT Λ Σ}.
 
-(* crashed(P) should hold if P holds after a crash step. *)
-Definition crashed (E: coPset) (P: iProp Σ) : iProp Σ :=
-  (∀ σ1 σ2, state_interp σ1 ∗ ⌜crash_step Λ.(sem) σ1 σ2 tt⌝ ={E,∅,∅}▷=∗ P ∗ state_interp σ2)%I.
+(** crashed(P) should hold if P must hold after a crash step.
 
-Global Instance crashed_ne E n :
-  Proper (dist n ==> dist n) (crashed E).
+   The intuition is that if we are given ownership of all resources needed to
+   prove the new state interpretation and the crash interpretation, then we
+   should be able to derive the state interpretation and P. This should work for
+   something like the encoding of state used in the 'heap_lang' Iris example.
+
+   As part of an adequacy proof, we will just have to show that for all such σ1 σ2,
+   there exists a Q as below.
+
+   TODO: maybe the thing to the left of the implication should be under a □ modality.
+   it would simplify the meta-theory and will probably work
+ *)
+
+Definition crashed (P: iProp Σ) : iProp Σ :=
+  (∀ σ1 σ2 Q,
+      (Q ∗ state_interp σ1 ∗ ⌜crash_step Λ.(sem) σ1 σ2 tt⌝ ==∗ state_interp σ2 ∗ crash_interp σ1 σ2)
+    → (Q ∗ state_interp σ1 ∗ ⌜crash_step Λ.(sem) σ1 σ2 tt⌝ ==∗ state_interp σ2 ∗ P))%I.
+
+
+(* Alternative possible definition, but it seems too awkward to work with *)
+
+(*
+Definition crashed (E: coPset) (P: iProp Σ) : iProp Σ :=
+  (∀ σ1 σ2 Q, (Q ∗ state_interp σ1 ∗ ⌜crash_step Λ.(sem) σ1 σ2 tt⌝ ={E,∅,∅}▷=∗ state_interp σ2)
+    → (Q ∗ state_interp σ1 ∗ ⌜crash_step Λ.(sem) σ1 σ2 tt⌝ ={E,∅,∅}▷=∗ P ∗ state_interp σ2))%I.
+*)
+
+
+Global Instance crashed_ne n :
+  Proper (dist n ==> dist n) (crashed).
 Proof. rewrite /crashed => P Q Hequiv. repeat f_equiv; eauto. Qed.
 
-Global Instance crashed_proper E:
-  Proper ((≡) ==> (≡)) (crashed E).
+Global Instance crashed_proper:
+  Proper ((≡) ==> (≡)) (crashed).
 Proof. intros ?? Hequiv. apply equiv_dist=>n; apply crashed_ne; auto. Qed. 
 
-Lemma crashed_mono E P Q :
-  crashed E P -∗ (P ==∗ Q) -∗ crashed E Q.
+Lemma crashed_mono P Q :
+  (P -∗ Q) →
+  crashed P -∗ crashed Q.
 Proof.
-  iIntros "Hc HPQ". iIntros (σ1 σ2) "H".
-  iMod ("Hc" $! σ1 σ2 with "H") as "Hc".
-  iModIntro. iNext. iMod "Hc" as "(?&?)".
-  iMod ("HPQ" with "[$]"). iModIntro. iFrame. 
-Qed.
-      
-Lemma fupd_crashed_strong E1 E2 P:
-  (|={E2, E1}=> crashed E1 P) -∗ crashed E2 P.
-Proof.
-  iIntros "Hc". iIntros (σ1 σ2) "H".
-  iMod "Hc". by iApply "Hc".
-Qed.
-  
-Lemma crashed_plainly E P Q:
-  crashed E P ∗ ■ Q -∗ crashed E (P ∗ ■ Q).
-Proof.
-  iIntros "(Hc&HQ)".
-  iIntros (σ1 σ2) "H".
-  iMod ("Hc" $! σ1 σ2 with "H").
-  iModIntro. iFrame; auto.
+  iIntros (HPQ).
+  iIntros "Hc". iIntros (σ1 σ2 Q').
+  iSpecialize ("Hc" $! σ1 σ2 Q').
+  iRevert "Hc".
+  iApply impl_mono; auto. by rewrite HPQ.
 Qed.
 
-Lemma fupd_crashed E P: (|={E}=> crashed E P) -∗ crashed E P.
-Proof. iApply fupd_crashed_strong. Qed.
-
-Lemma crashed_fupd E P: crashed E (|={∅}=> P) -∗ crashed E P.
+(* TODO: this should be upstreamed. *)
+Lemma and_curry: ∀ (PROP : bi) (P Q R : PROP), (P → Q → R)%I ≡ (P ∧ Q → R)%I.
 Proof.
-  iIntros "Hc". iIntros (σ1 σ2) "H".
-  iMod ("Hc" $! σ1 σ2 with "H") as "Hc".
-  iModIntro. iNext. by iMod "Hc" as "(>$&$)".
+  intros.
+  apply (anti_symm (⊢)).
+  - apply impl_intro_r.
+    rewrite and_assoc. by do 2 rewrite impl_elim_l.
+  - do 2 apply impl_intro_r. rewrite -and_assoc. apply impl_elim_l.
 Qed.
+
+Lemma crashed_plainly P Q:
+  crashed P ∗ ■ Q -∗ crashed (P ∗ ■ Q).
+Proof.
+  iIntros "(Hc&#HQ)".
+  iIntros (σ1 σ2 Q').
+  iSpecialize ("Hc" $! σ1 σ2 Q').
+  iRevert "Hc".
+  (* TODO: write a tactic to automatically introduce an implication when the
+  spatial context contains 1 assertion *)
+  rewrite -impl_wand_1 and_curry impl_elim_l.
+  iIntros "H1 H2".
+  iFrame "HQ". iMod ("H1" with "H2").
+  iModIntro; auto.
+Qed.
+
+Lemma crash_interp_crashed P:
+  (∀ σ1 σ2, crash_interp σ1 σ2 ==∗ P) →
+  crashed P.
+Proof.
+  intros Hci. iIntros (σ1 σ2 Q) "H1 H2".
+  iMod ("H1" with "H2") as "(?&?)". iMod (Hci with "[$]"). iModIntro; iFrame.
+Qed.
+
 End crash.
